coq/Utils.v
@@ -5,6 +5,9 @@ Unset Strict Implicit.
 Unset Printing Implicit Defensive.
 Set Bullet Behavior "Strict Subproofs".
 
+(***************
+ Tactics 
+****************)
 
 Tactic Notation "intro_to" constr(ty) :=
   repeat match goal with
@@ -28,3 +31,45 @@ Ltac construct_with t :=
 Tactic Notation "inversion" :=
   let H := fresh in
   move => H; inversion H.
+
+
+(****************
+Definitions
+*****************)
+
+(* grouped right with the fixpoint for better decreasing argument analysis*)
+Definition all2 := 
+fun (S T : Type) (r : S -> T -> bool) =>
+fix all2 (s : seq S) (t : seq T) {struct s} : bool :=
+  match s, t with
+  | [::], [::] => true
+  | x :: s0, y::t0 => r x y && all2 s0 t0
+  | _,_ => false
+  end.
+
+Lemma all2P {T} eqb (l1 l2 : seq T)
+  : (forall e1 e2, reflect (e1 = e2) (eqb e1 e2)) ->
+    reflect (l1 = l2) (all2 eqb l1 l2).
+Proof.
+  move => eqbP.
+  elim: l1 l2.
+  - case; simpl; [by constructor|].
+    intros.
+    constructor; eauto.
+    move => H; inversion H.
+  - move => a l IH.
+    case; simpl.
+    constructor; move => H; inversion H.
+    intros.
+    move: (eqbP a a0).
+    case (eqb a a0); simpl.
+    move: (IH l0); case:(all2 eqb l l0); simpl.
+    + constructor.
+      inversion IH0; inversion eqbP0; by subst.
+    + constructor.
+      move => lfl.
+      inversion lfl.
+      inversion IH0; eauto.
+    + constructor; move => lfl.
+      inversion lfl; inversion eqbP0; auto.
+Qed.
